\begin{exercise}
Let \(\left(\left(A_\sigma\right),\left\llbracket\_\right\rrbracket\right)\) be a \(\Sigma\)-model and \(\rho\) a valuation \(\left(X_\sigma \to A_\sigma\right)\).
\begin{parts}
\part
Show that
\begin{equation*}
\left\llbracket M\left[N/x\right]\right\rrbracket_\rho
= \left\llbracket M\right\rrbracket_{\rho(x \mapsto \left\llbracket N\right\rrbracket_\rho)}.
\end{equation*}
\part
Let \(\left(\left(B_\sigma\right),\left\llbracket\_\right\rrbracket\right)\) be another \(\Sigma\)-model and \(H_\sigma : A_\sigma \to B_\sigma\) be a morphism of \(\Sigma\)-models (\emph{i.e.} a morphism in the fibre of \(\SModel\) over \(\Sigma\)).
Show that
\begin{equation*}
H\left(\left\llbracket M \right\rrbracket_\rho\right)
= \left\llbracket M \right\rrbracket_{H \circ \rho}.
\end{equation*}
\end{parts}
\end{exercise}

\begin{partsolution}{i}
We proceed by induction on terms.
First, for \(\tau\in T\), \(x, y \in X_\tau\), and \(N \in \Terms_\tau(X)\),
\begin{align*}
\left\llbracket y\left[N/x\right]\right\rrbracket_\rho^\tau
&=\begin{cases}
\left\llbracket N\right\rrbracket_\rho^\tau & \text{if \(y = x\)} \\
\left\llbracket y\right\rrbracket_\rho^\tau & \text{otherwise}
\end{cases} \\
&=\begin{cases}
\left\llbracket N\right\rrbracket_\rho^\tau & \text{if \(y = x\)} \\
\rho_\tau(y) & \text{otherwise}
\end{cases} \\
&= \rho_\tau(x \mapsto \left\llbracket N\right\rrbracket_\rho^\tau)(y) \\
&=\left\llbracket y\right\rrbracket_{\rho(x \mapsto \left\llbracket N\right\rrbracket_\rho^\tau)}^\tau.
\end{align*}
Next, if \(\tau_0,\ldots,\tau_n\in T\), \(M_0 \in \Terms_{\tau_0}(X), \ldots, M_{n-1} \in \Terms_{\tau_{n-1}}(X)\), and \(F : \tau_0,\,\ldots,\,\tau_{n-1} \to \tau_n\) is a function symbol in \(\Sigma\), then, by induction,
\begin{align*}
&\left\llbracket F(M_0,\ldots,M_{n-1})\left[N/x\right]\right\rrbracket_\rho^{\tau_n} \\
&\qquad=\left\llbracket F(M_0\left[N/x\right],\ldots,M_{n-1}\left[N/x\right])\right\rrbracket_\rho^{\tau_n} \\
&\qquad=\left\llbracket F\right\rrbracket\left(\left\llbracket M_0\left[N/x\right]\right\rrbracket_\rho^{\tau_0},\ldots,\left\llbracket M_{n-1}\left[N/x\right]\right\rrbracket_\rho^{\tau_{n-1}}\right) \\
&\qquad=\left\llbracket F\right\rrbracket\left(\left\llbracket M_0\right\rrbracket_{\rho(x \mapsto \left\llbracket N\right\rrbracket_\rho^\tau)}^{\tau_0},\ldots,\left\llbracket M_{n-1}\right\rrbracket_{\rho(x \mapsto \left\llbracket N\right\rrbracket_\rho^\tau)}^{\tau_{n-1}}\right) \\
&\qquad=\left\llbracket F(M_0,\ldots,M_{n-1})\right\rrbracket_{\rho(x \mapsto \left\llbracket N\right\rrbracket_\rho^\tau)}^{\tau_n}.
\qedhere
\end{align*}
\end{partsolution}
